src/DepList.v
@@ -3,6 +3,15 @@ Require Export EquivDec.
 
 Set Implicit Arguments.
 
+Theorem EquivDec_refl_left (T : Type) {c : EqDec T (@eq T)} :
+  forall (n : T), equiv_dec n n = left (refl_equal _).
+Proof.
+  intros. destruct (equiv_dec n n); try congruence.
+  Require Eqdep_dec.
+  rewrite (Eqdep_dec.UIP_dec (A := T) (@equiv_dec _ _ _ c) e (refl_equal _)).
+  reflexivity.
+Qed.
+
 Class SemiDec (t : Type) : Type :=
 { seq_dec : forall a b : t, option (a = b) }.
 Global Instance EquivDec_SemiDec t (EQ : EqDec t (@eq t)) : SemiDec t :=
@@ -48,7 +57,6 @@ Global Instance SemiDec_list T (S : SemiDec T) : SemiDec (list T) :=
     | _ , _ => None
   end
 }.
-
 
 Inductive dcomp T (a b : T) : Type :=
 | Lt | Gt | Eq : a = b -> dcomp a b.
